lean/Splay/AssocCorrect.lean
@@ -1,0 +1,164 @@
+-- proving that the association lists are correct using a basic map
+import Mathlib.Tactic.Linarith
+
+import Splay.Assoc
+import Splay.Tactics
+
+def Map (α : Type) := Nat -> Option α
+
+@[simp]
+def insert_map {α : Type} (m : Map α) (k : Nat) (v : α) :=
+  fun k' => if k' = k then some v else m k'
+
+@[simp]
+def union_map {α : Type} (m1 m2 : Map α) :=
+  fun k' =>
+    match m1 k' with
+    | none => m2 k'
+    | x => x
+
+@[simp]
+def bound_map {α : Type} (m : Map α) (k : Nat) :=
+  match m k with
+  | none => false
+  | some _ => true
+
+@[simp]
+def lookup_map {α : Type} (m : Map α) (k : Nat) := m k
+
+@[simp]
+def empty_map {α : Type} : Map α := fun _ => none
+
+@[simp]
+def map_of_list {α : Type} (l : Assoc α) : Map α :=
+  match l with
+  | .nil => empty_map
+  | .cons (k, v) tl => insert_map (map_of_list tl) k v
+
+@[simp]
+def abs_assoc {α : Type} (l : Assoc α) : Map α := map_of_list l
+-- this def doesn't work because of universes?
+-- @[simp]
+-- def abs_assoc {α : Type u} (l : Assoc α) :=
+--   l.foldl (fun m (k, v) => fun k' => if k' = k then some v else m k') (fun _ => none)
+
+-- TODO assoc α doesn't work with app (++)
+theorem abs_assoc_app {α : Type} (l1 l2 : List (Nat × α)) :
+  abs_assoc (l1 ++ l2) = union_map (abs_assoc l1) (abs_assoc l2) := by
+  funext k
+  induction l1 with
+  | nil => simp
+  | cons elt l1 ihl1 =>
+    cases elt
+    rename_i k' v'
+    simp
+    by_cases' (k = k') heq
+    unfold abs_assoc at ihl1
+    rw [ihl1]
+    rfl
+
+theorem bound_relate {α : Type} (l : Assoc α) (k : Nat) :
+  bound_map (abs_assoc l) k = bound_assoc l k := by
+  induction l with
+  | nil => simp
+  | cons elt l ihl =>
+    cases elt
+    rename_i k' v'
+    simp
+    by_cases' (k = k') heq
+    rw [<- ihl]
+    have heq2 : ¬k' = k := by -- TODO dumb... is there a tactic that can handle this?
+      intro hasdf
+      apply heq
+      rw [hasdf]
+    simp [*]
+
+theorem lookup_relate {α : Type} (l : Assoc α) (k : Nat) :
+  lookup_map (abs_assoc l) k = lookup_assoc l k := by
+  induction l with
+  | nil => simp
+  | cons elt l ihl =>
+    cases elt
+    rename_i k' v'
+    simp
+    by_cases' (k = k') heq
+    rw [<- ihl]
+    have heq2 : ¬k' = k := by -- TODO dumb... is there a tactic that can handle this?
+      intro hasdf
+      apply heq
+      rw [hasdf]
+    simp [*]
+
+theorem insert_relate {α : Type} (l : Assoc α) (k : Nat) (v : α) :
+  insert_map (abs_assoc l) k v = abs_assoc (insert_assoc l k v) := by
+  induction l with
+  | nil => simp
+  | cons elt l ihl =>
+    funext k0
+    cases elt
+    rename_i k' v'
+    simp
+    by_cases' (k < k') hlt
+    by_cases' (k > k') hgt
+    case pos =>
+      by_cases' (k0 = k) heq0
+      case pos =>
+        have hneq : k ≠ k' := by linarith
+        simp [*]
+        unfold abs_assoc at ihl
+        rw [<-ihl]
+        simp [*]
+      case neg =>
+        by_cases' (k0 = k') heq'
+        unfold abs_assoc at ihl
+        rw [<-ihl]
+        simp [*]
+    case neg =>
+      have heq' : k = k' := by linarith
+      by_cases' (k0 = k) heq0
+      subst heq'
+      simp [*]
+
+-- algebraic specification
+-- 1. ∀ k, lookup_assoc empty_assoc k = none
+-- 2. ∀ k v l, lookup_assoc (insert_assoc l k v) k = some v
+-- 3. ∀ k k' v l, k' ≠ k -> lookup_assoc (insert_assoc l k v) k' = lookup_assoc l k'
+
+-- TODO how to apply the time to empty_assoc even though it's implicit?
+-- theorem lookup_assoc_empty {α : Type} (k : Nat) : lookup_assoc empty_assoc k = none := by simp
+
+theorem lookup_assoc_eq (α : Type) (k : Nat) (v : α) (l : Assoc α) :
+  lookup_assoc (insert_assoc l k v) k = some v := by
+  induction l with
+  | nil => simp
+  | cons elt l ihl =>
+    cases elt
+    rename_i k' v'
+    simp
+    by_cases' (k < k') hlt
+    by_cases (k > k')
+    case pos =>
+      rename_i hgt
+      simp [hgt]
+      have hne : k' ≠ k := by linarith
+      simp [*]
+    case neg =>
+      have heq : k' = k := by linarith
+      subst heq
+      simp
+
+theorem lookup_assoc_neq {α : Type} (k k' : Nat) (v : α) (l : Assoc α) :
+  k ≠ k' ->
+  lookup_assoc (insert_assoc l k v) k' = lookup_assoc l k' := by
+  intro h
+  induction l with
+  | nil => simp [h]
+  | cons elt l ihl =>
+    cases elt
+    rename_i k0 v0
+    simp
+    by_cases' (k < k0) hlt
+    by_cases' (k > k0) hgt
+    have heq : k = k0 := by linarith
+    subst heq
+    simp [*]
