lean/Splay/AssocRelate.lean
@@ -1,0 +1,347 @@
+import Mathlib.Tactic.Linarith
+
+import Splay.Assoc
+import Splay.Tactics
+import Splay.STree
+import Splay.BST
+
+@[simp]
+def STree.abs {α : Type} (t : STree α) : Assoc α := t.elements
+
+theorem elements_splay_impl {α : Type} (t : STree α) (key : Nat) (hbst : BST t)
+  : t.elements = (t.splay key).elements := by
+  induction t using STree.inductionOn with
+  | base => simp
+  | ind_te k v => simp
+  | ind_tl k v ll lk lv lr ihll ihlr =>
+    simp
+    by_cases' (key = k) heq
+    by_cases' (key < k) hlt
+    by_cases' (key = lk) heqlk
+    by_cases' (key < lk) hltlk
+    case pos =>
+      cases hdes : ll.splay key with
+      | leaf => simp
+      | node lll llk llv llr =>
+        rw [hdes] at ihll
+        simp at *
+        rw [ihll]
+        simp
+        cases hbst
+        rename_i hbstl _ _ _
+        cases hbstl
+        assumption
+    case neg =>
+      cases hdes : lr.splay key with
+      | leaf => simp
+      | node lrl lrk lrv lrr =>
+        rw [hdes] at ihlr
+        simp at *
+        rw [ihlr]
+        simp
+        cases hbst
+        rename_i hbstl _ _ _
+        cases hbstl
+        assumption
+  | ind_tr k v rl rk rv rr ihrl ihrr =>
+    simp
+    by_cases' (key = k) heq
+    by_cases' (key < k) hlt
+    by_cases' (key = rk) heqrk
+    by_cases' (key < rk) hltrk
+    case pos =>
+      cases hdes : rl.splay key with
+      | leaf => simp
+      | node rll rlk rlv rlr =>
+        rw [hdes] at ihrl
+        simp at *
+        rw [ihrl]
+        simp
+        cases hbst
+        rename_i hbstr _
+        cases hbstr
+        assumption
+    case neg =>
+      cases hdes : rr.splay key with
+      | leaf => simp
+      | node rrl rrk rrv rrr =>
+        rw [hdes] at ihrr
+        simp at *
+        rw [ihrr]
+        cases hbst
+        rename_i hbstr _
+        cases hbstr
+        assumption
+  | ind k v ll lk lv lr rl rk rv rr ihll ihlr ihrl ihrr =>
+    simp
+    by_cases' (key = k) heq
+    by_cases' (key < k) hlt
+    case pos =>
+      by_cases' (key = lk) heqlk
+      by_cases' (key < lk) hltlk
+      case pos =>
+        cases hdes : ll.splay key with
+        | leaf => simp
+        | node lll llk llv llr =>
+          rw [hdes] at ihll
+          simp at *
+          rw [ihll]
+          simp
+          cases hbst
+          rename_i hbstl _ _ _
+          cases hbstl
+          assumption
+      case neg =>
+        cases hdes : lr.splay key with
+        | leaf => simp
+        | node lrl lrk lrv lrr =>
+          rw [hdes] at ihlr
+          simp at *
+          rw [ihlr]
+          simp
+          cases hbst
+          rename_i hbstl _ _ _
+          cases hbstl
+          assumption
+    case neg =>
+      by_cases' (key = rk) heqrk
+      by_cases' (key < rk) hltrk
+      case pos =>
+        cases hdes : rl.splay key with
+        | leaf => simp
+        | node rll rlk rlv rlr =>
+          rw [hdes] at ihrl
+          simp at *
+          rw [ihrl]
+          simp
+          cases hbst
+          rename_i hbstr _
+          cases hbstr
+          assumption
+      case neg =>
+        cases hdes : rr.splay key with
+        | leaf => simp
+        | node rrl rrk rrv rrr =>
+          rw [hdes] at ihrr
+          simp at *
+          rw [ihrr]
+          cases hbst
+          rename_i hbstr _
+          cases hbstr
+          assumption
+
+---- helpers for the rest
+theorem pull_cons_from_if {α : Type} {b1 : Prop} {b2 : Prop} [Decidable b1] [Decidable b2] (a : α) (l1 l2 l3 : List α)
+  : a :: (if b1 then l1 else if b2 then l2 else l3) = if b1 then a :: l1 else if b2 then a :: l2 else a :: l3 := by
+  by_cases b1 <;> simp [*]
+  by_cases b2 <;> simp [*]
+
+theorem bound_assoc_not (l : Assoc α) (k : Nat)
+  : Forall (fun x => x.1 ≠ k) l -> bound_assoc l k = false := by
+  induction l with
+  | nil => simp
+  | cons e t ih =>
+    intro h
+    cases h
+    simp [*]
+
+theorem bound_assoc_split {α : Type} (k k' : Nat) (v' : α) (l1 l2 : Assoc α)
+  : Forall (fun (k0, _) => k0 < k') l1 ->
+    Forall (fun (k0, _) => k0 > k') l2 ->
+    bound_assoc (l1 ++ (k', v') :: l2) k =
+    if k < k' then
+      bound_assoc l1 k
+    else if k > k' then
+      bound_assoc l2 k
+    else true := by
+  induction l1 with
+  | nil =>
+    simp
+    intros _ h2
+    by_cases' (k < k') hlt
+    apply And.intro
+    linarith
+    apply bound_assoc_not
+    apply Forall_imp
+    apply h2
+    intros
+    linarith
+    by_cases' (k' < k) hgt
+    have hneq : k' ≠ k := by linarith
+    simp [*]
+    have heq : k' = k := by linarith
+    simp [*]
+  | cons e l1 ih =>
+    simp at *
+    intros h1 h2
+    cases h1
+    rename_i hlte h1
+    by_cases' (k < k') hlt
+    by_cases' (k' < k) hgt
+    have hneq : e.1 ≠ k := by linarith
+    simp [*]
+
+theorem lookup_assoc_not (l : Assoc α) (k : Nat)
+  : Forall (fun x => x.1 ≠ k) l -> lookup_assoc l k = none := by
+  induction l with
+  | nil => simp
+  | cons e t ih =>
+    intro h
+    cases h
+    simp [*]
+
+-- TODO combine these three, terrible
+theorem lookup_assoc_split (k k' : Nat) (v' : α) (l1 l2 : Assoc α)
+  : Forall (fun (k0, _) => k0 < k') l1 ->
+    Forall (fun (k0, _)     => k0 > k') l2 ->
+    lookup_assoc (l1 ++ (k', v') :: l2) k =
+    if k < k' then
+      lookup_assoc l1 k
+    else if k > k' then
+      lookup_assoc l2 k
+    else some v' := by
+  induction l1 with
+  | nil =>
+    simp
+    intro _ h2
+    by_cases' (k < k') hlt
+    have hneq : k' ≠ k := by linarith
+    simp [*]
+    apply lookup_assoc_not
+    apply Forall_imp
+    apply h2
+    intros
+    linarith
+    by_cases' (k' < k) hgt
+    have hneq : k' ≠ k := by linarith
+    intros
+    contradiction
+    have heq : k' = k := by linarith
+    simp [*]
+  | cons e l1 ih =>
+    simp at *
+    intros h1 h2
+    cases h1
+    rename_i hlte h1
+    by_cases' (k < k') hlt
+    by_cases' (k' < k) hgt
+    intros
+    exfalso
+    linarith
+    intros
+    exfalso
+    linarith
+
+-- TODO try to make this more generic so that it applies to the other guys?
+theorem insert_assoc_split {α : Type} (k k' : Nat) (v v' : α) (l1 l2 : Assoc α)
+  : Forall (fun (k0, _) => k0 < k') l1 ->
+    Forall (fun (k0, _)     => k0 > k') l2 ->
+    insert_assoc (l1 ++ (k', v') :: l2) k v =
+    if k < k' then
+      (insert_assoc l1 k v) ++ (k', v') :: l2
+    else if k > k' then
+      l1 ++ (k', v') :: insert_assoc l2 k v
+    else
+      l1 ++ (k, v) :: l2 := by
+  induction l1 with
+  | nil => simp
+  | cons h l1 ihl =>
+    intros hl hr
+    cases h
+    rename_i kl vl
+    cases hl
+    rename_i hlt1 hfl
+    simp at *
+    by_cases' (k < kl) hlt
+    case pos =>
+      have hlt2 : k < k' := by linarith
+      simp [*]
+    case neg =>
+      rw [<-ihl]
+      simp [*]
+      by_cases' (kl < k) hgt
+      rw [<-pull_cons_from_if]
+      have heq : kl = k := by linarith
+      subst heq
+      simp [*]
+      apply hfl
+      apply hr
+
+theorem bound'_relate {α : Type} (t : STree α) (key : Nat) (hbst : BST t)
+  : t.bound' key = bound_assoc t.abs key := by
+  induction hbst with
+  | leaf => simp
+  | node l k v r hfl hfr hbstl hbstr ihl ihr =>
+    simp
+    have hfal : Forall (fun (k', _) ↦ k' < k) l.elements := by
+      rw [Forall_relate] at hfl
+      apply hfl
+    have hfar : Forall (fun (k', _) ↦ k' > k) r.elements := by
+      rw [Forall_relate] at hfr
+      apply hfr
+    rw [bound_assoc_split] <;> try assumption
+    by_cases' (key = k) heq
+    by_cases' (key < k) hlt
+    have hgt : k < key := by apply obvious_arith <;> assumption
+    simp [*]
+
+theorem bound_relate_impl {α : Type} (t : STree α) (k : Nat) (hbst : BST t)
+  : t.bound k = bound_assoc t.abs k := by
+  rw [splay_bound_equiv]
+  apply bound'_relate t k hbst
+
+theorem lookup'_relate {α : Type} (t : STree α) (key : Nat) (hbst : BST t)
+  : (t.lookup' key).1 = lookup_assoc t.abs key := by
+  induction hbst with
+  | leaf => simp
+  | node l k v r hfl hfr hbstl hbstr ihl ihr =>
+    simp
+    have hfal : Forall (fun (k', _) ↦ k' < k) l.elements := by
+      rw [Forall_relate] at hfl
+      apply hfl
+    have hfar : Forall (fun (k', _) ↦ k' > k) r.elements := by
+      rw [Forall_relate] at hfr
+      apply hfr
+    rw [lookup_assoc_split] <;> try assumption
+    by_cases' (key = k) heq
+    by_cases' (key < k) hlt
+    case pos =>
+      apply ihl
+    case neg =>
+      have hgt : k < key := by apply obvious_arith <;> assumption
+      simp [*]
+      apply ihr
+
+theorem lookup_relate_impl {α : Type} (t : STree α) (k : Nat) (hbst : BST t)
+  : (t.lookup? k).1 = lookup_assoc t.abs k := by
+  rw [splay_lookup_equiv]
+  apply lookup'_relate t k hbst
+
+theorem ins_relate {α : Type} (t : STree α) (key : Nat) (val : α) (hbst : BST t)
+  : (t.ins key val).abs = insert_assoc t.abs key val := by
+  induction hbst with
+  | leaf => simp
+  | node l k v r hfl hfr hbstl hbstr ihl ihr =>
+    simp
+    have hfal : Forall (fun (k', _) ↦ k' < k) l.elements := by
+      rw [Forall_relate] at hfl
+      apply hfl
+    have hfar : Forall (fun (k', _) ↦ k' > k) r.elements := by
+      rw [Forall_relate] at hfr
+      apply hfr
+    rw [insert_assoc_split] <;> try assumption
+    by_cases' (key = k) heq
+    by_cases' (key < k) hlt
+    case pos =>
+      apply ihl
+    case neg =>
+      have hgt : key > k := by apply obvious_arith <;> assumption
+      simp [*]
+      apply ihr
+
+theorem insert_relate_impl {α : Type} (t : STree α) (k : Nat) (v : α) (hbst : BST t)
+  : (t.insert k v).abs = insert_assoc t.abs k v := by
+  simp
+  rw [<-elements_splay_impl]
+  . apply ins_relate t k v hbst
+  . apply ins_BST t k v hbst
